KeyManagement/Automation.v
@@ -1,0 +1,26 @@
+From Coq Require Import
+     String
+     Sumbool
+     Eqdep.
+
+Require Import
+        MyPrelude
+        Tactics
+        Maps.
+
+Require Import RealWorld.
+
+Set Implicit Arguments.
+
+
+
+Ltac solve_findUserKeys_rewrites :=
+  repeat
+    match goal with
+    | [ |- context [RealWorld.user_keys] ] => unfold RealWorld.user_keys
+    | [ |- context [ _ $? _] ] => progress clean_map_lookups
+    | [ |- context [match _ $? _ with _ => _ end]] => context_map_rewrites
+    end; simpl; trivial.
+
+Hint Rewrite @findUserKeys_readd_user_same_keys_idempotent' using solve [ solve_findUserKeys_rewrites ] : find_user_keys.
+Hint Rewrite @findUserKeys_readd_user_addnl_keys using solve [ solve_findUserKeys_rewrites ] : find_user_keys.
